spec/Rchain.lean
@@ -1,2 +1,6 @@
 import Rchain.Syntax
+import Rchain.Par
+import Rchain.Cmp
+import Rchain.Rho
 import Rchain.Sort
+import Rchain.Ty
